coq/theories/verification.v
@@ -10,8 +10,12 @@ Module Type Verif_Domain.
         -   The bucchi automaton [i_aut] describes the input of the system.
         -   The bucchi automaton [o_aut] describes the expected state of 
             the system 
-        We assume that in both automata, each node has at least a sucessor *)
- 
+        We assume that in both automata, each node has at least one sucessor.
+    *)
+
+    Definition successor {N L : Type} (a: automaton N L) := forall n,
+        reachable a n -> exists p m, transition a n p m.
+
     Parameter input state : Set.
 
     Parameter program : input * state -> state.
@@ -23,18 +27,15 @@ Module Type Verif_Domain.
     Parameter i_aut : automaton node1 (input -> Prop).
     Parameter o_aut : automaton node2 (input * state -> Prop).
 
-    Parameter i_aut_successors : 
-        forall n, reachable i_aut n -> 
-            exists g m, transition i_aut n g m.
+    Parameter i_aut_successor : successor i_aut.
+    Parameter o_aut_successor : successor o_aut.
 
-    Parameter o_aut_successors : 
-        forall n, reachable o_aut n -> 
-            exists g m, transition o_aut n g m.
+    Definition sat {A} := fun (p : A -> Prop) (x : A) => p x.
 
-    Notation i_step_type := ((input -> Prop) * node1).
-    Notation o_step_type := ((input * state -> Prop) * node2).
-    Notation i_path_type := (list i_step_type).
-    Notation o_path_type := (list o_step_type).
+    Definition i_step_type := ((input -> Prop) * node1)%type.
+    Definition o_step_type := ((input * state -> Prop) * node2)%type.
+    Definition i_path_type := list i_step_type.
+    Definition o_path_type := list o_step_type.
 
 End Verif_Domain.
                     
@@ -45,47 +46,18 @@ Module Verif (Import D : Verif_Domain).
     Definition update (st : input * state) (i : input) : input * state :=
         (i, snd st).
 
-    (** The function [freeze] makes a input * state predicate independent
-        of the value of the input by quantifying them existentially *)
-
-    Definition freeze (p : input * state -> Prop) : input * state -> Prop :=
-        fun (st : input * state
-) => let (i,o) := st in exists i, p (i,o).
-
-    Lemma freeze_prop : 
-        forall (p : input * state
- -> Prop) (st : input * state
- ), p st -> freeze p st.
-    Proof.
-        intros.
-        destruct st as [i o].
-        exists i.
-        exact H.
-    Qed.
-        
-    Lemma freeze_prop2 : 
-        forall p st i, freeze p st -> freeze p (update st i).
-    Proof.
-        intros.
-        unfold freeze in *.
-        destruct st as [i0 o0].
-        simpl.
-        auto.
-    Qed.
         
     (** We define the product automaton of i_aut and o_aut *)
 
     Definition io_aut := product i_aut o_aut.
 
-    Notation io_step_type := 
-        ((input -> Prop) * (input * state
- -> Prop) * (node1 * node2)).
-    Notation io_path_type := (list io_step_type ).
+    Definition io_step_type := ((input -> Prop) * (input * state -> Prop) * (node1 * node2))%type.
+    Definition io_path_type := list io_step_type.
 
-    (** Obviously, in the product automaton, each node as a least a successor *)
+    (** Obviously, in the product automaton, each node as at least one successor *)
 
-    Lemma io_aut_successors : 
-        forall n, reachable io_aut  n -> 
+    Lemma io_aut_successor : 
+        forall n, reachable io_aut n -> 
             exists g m, transition io_aut n g m.
     Proof.
         intros.
@@ -99,43 +71,70 @@ Module Verif (Import D : Verif_Domain).
         assert (reachable_from o_aut (init o_aut) (snd n)).
         {
             destruct n.
-            apply reachable_right_proj in H.
+            apply reachable_right_proj in H.  
             apply H.
         }
-        apply i_aut_successors in H0.
-        apply o_aut_successors in H1.
-        destruct H0 as [f [n1 Ha]].
-        destruct H1 as [g [m1 Hb]].
+        apply i_aut_successor in H0 as [f [n1 Ha]].
+        apply o_aut_successor in H1 as [g [m1 Hb]].
         exists (f,g), (n1,m1).
         split; assumption.
     Qed. 
         
-    (* il doit y avoir un successeur par f *)
-    (* le noeud doit être accessible *)
 
     (** Now we define the constraints that should be satisfied 
         by nodes of the product automaton which are assumed to 
         be checked by an external tool *)
 
-    Definition next_gen (n : node1 * node2) (f : input -> Prop) 
-        (n' : node1) : input * state -> Prop := 
-            fun x => exists g m, transition io_aut n (f,g) (n',m) /\ g x.
 
-    Definition prev_gen (n : node1 * node2) : input * state -> Prop :=
-        fun x => exists f g m, transition io_aut m (f,g) n /\ g x.
+    (** Given a node [n] from [io_aut] and a node [m_i] from [i_aut], there must exist a node [m_o] from [o_aut]
+        which together form the successor [(m_i,m_o)] of [n] in [io_aut].
+        In addition, the transition from [n] to [m] is labeled by (f,g) 
+        where g holds for a certain pair of input and state [x].
+    *)
+    Definition next_gen (n : node1 * node2) (f : input -> Prop)  : input * state -> Prop := 
+            fun x => exists g m, transition io_aut n (f,g) m /\ g x.
 
+    (** Given a node [m] from [io_aut], there must exist a node [n] which is a precedessor of [m].
+        In addition, the transition from [n] to [m] is labeled by (f,g)  where g holds an 
+        for a certain unknown input and a known state [st].
+     *)
+    Definition prev_gen (m : node1 * node2) : state -> Prop :=
+        fun st => exists f g n, transition io_aut n (f,g) m /\ exists i, g (i,st).
+
+    (** The initial node [n] is valid iff given : 
+    
+        - any predicate on input [f] making up the first part of the label of at least one transition exiting [n] 
+        - any input [i] for which [f] holds 
+        - any state [st] respecting P_init, i.e. a valid initial state
+
+        there exists a transition from [n] labeled by ([f],[g])
+        where g holds for [i] and the next state of the program.
+
+        That is to say, given an initial state and input, any immediately following state produced 
+        by the system is correct
+    *)
     Definition validInit := 
-        forall (f : input -> Prop) (n : node1) (i : input) (st:state),
+        forall (f : input -> Prop) (i : input) (st:state),
             (exists g m, transition io_aut (init io_aut) (f,g) m ) ->
-            P_init st -> f i -> next_gen (init io_aut) f n (i, program (i,st)).
+            P_init st -> f i -> next_gen (init io_aut) f (i, program (i,st)).
 
+
+    (** A node [n] is valid iff given :
+        - any predicate on input [f] making up the first part of the label of at least one transition exiting [n]
+        - any input [i] for which [f] holds 
+        - any state [st] for which   
+
+        there exists a transition labeled (f,_) from the initial state to some other state, then
+
+    *)
     Definition validNode (n : node1 * node2) :=
-        forall (f : input -> Prop) (n0 : node1) (i :input) (st : state),
+        forall (f : input -> Prop) (i :input) (st : state),
             (exists g m, transition io_aut n (f,g) m ) ->
-            freeze (prev_gen n) (i,st) -> f i ->
-            next_gen n f n0 (i, program (i,st)).
+            prev_gen n st -> f i ->
+            next_gen n f (i, program (i,st)).
         
-    Definition validAutomata := 
+
+    Definition validAutomaton := 
         validInit /\ (forall n, reachable io_aut n -> validNode n).
 
 End Verif.
@@ -144,80 +143,110 @@ Module Correctness (Import D : Verif_Domain).
 
     Module Import M := Verif D.    
 
-    Notation trace := (list (input * state)).
-    Notation inputs := (List.map (@fst input state)).
+    Definition trace := list (input * state).
+    Definition inputs := List.map (@fst input state).
+    Definition states := List.map (@snd input state).
 
+
+    (** A running system begins with an initial state. Then, when given an input, 
+        it produces a new state which stays the same until a new input is given to
+        produce a new state and so on. A trace is recorded which keeps an history of pairs of
+        received input and new state produced for this input.
+    *)
     Inductive run : D.state -> trace -> Prop :=
         | run_nil : forall st, run st nil
         | run_start : forall i st, 
-            run st (cons (i, D.program (i, st)) nil)
+            run st ((i, D.program (i, st))::nil)
         | run_cons : forall st i0 st0 i1 st1 l,
             run st ((i0,st0)::l) ->
             D.program (i1,st0) = st1 ->
             run st ((i1,st1)::(i0,st0)::l).
 
+
+    (** if we have a valid product automaton and an initial state [st],
+        for any run of the system begining with [st] and producing the trace [tr], 
+        for any path [ip] in the input automaton for which each input received by the system is correct,
+        there must exist a path in the product automaton whose left projection is [is] and 
+        whose right projection correspond to the fact each new state produced is correct.
+    *)
     Proposition correctness_aux : 
         forall (st : state) (tr : trace), 
-            validAutomata -> 
+            validAutomaton -> 
             D.P_init st -> run st tr -> 
-            forall is, language_w sat i_aut is (inputs tr) ->
-                exists p, left_proj p = is /\
-                    language_w sat_product io_aut p tr.
+            forall ip, language_wit sat i_aut ip (inputs tr) ->
+                exists p, left_proj p = ip /\ language_wit sat_product io_aut p tr.
     Proof.
         intros o_start tr [cond_init cond_node] o_start_valid run.
         induction run as 
             [ o_start | i0 o_start |  
                 o_start i_k o_k i_Sk o_Sk tr run tr_lang step ]; 
-        intros is input_lang; simpl in *.
-        -   replace is with (nil : list ((input -> Prop) * node1)) by
+        intros ipath input_lang; simpl in *.
+
+        -   replace ipath with (nil : list ((input -> Prop) * node1)) by
                 now rewrite (language_w_nil _ _ _ _ _ _ input_lang).
             exists nil.
             split; [reflexivity | apply language_empty].
+
         -   destruct input_lang as [H_path H_valid].
-            destruct is as [ | [f n1] is]; [ inversion H_valid |].
-            destruct is as [ | ];
-                inversion H_valid as [ | ? ? ? ? H_valid' ]; 
-                inversion H_valid'; subst.           
-            assert (transition i_aut (init i_aut) f n1 /\ sat f i0)
-                as [h_transition input_hd_is_valid] by
-                    now (inversion H_path; subst).
+            (** that the word [i0] is valid implies [is] is directly a transition from 
+                the initial node to [n1] labeled [f] such that [f] satisfies [i0].
+            *)
+            destruct ipath as [ | [f n1] ipath]; [ inversion H_valid |]. 
+            destruct ipath as [ | ]; inversion_clear H_valid as [ | ? ? ? ? [|] input_hd_is_valid]. 
+
+            assert (h_transition : transition i_aut (init i_aut) f n1) by now (inversion H_path; subst).
+
+
+            (** there must exist a transition in the product automaton from its initial node
+                to [(n1,m)] for a certain [m] labeled with [(f,g)] such that given 
+                the initial output [i0], the new state produced by the system is correct (g holds)  
+            *)
             assert (exists g m, 
                 transition io_aut (init i_aut, init o_aut) (f,g) (n1, m) /\ 
                     g (i0, program (i0, o_start))) as [g [m [Hu Hw]]].
             {
-                assert (next_gen (init D.i_aut, init D.o_aut) f n1 (i0, D.program (i0,o_start))) as H_next_gen.
-                {
-                    assert (exists (g : input * state
-             -> Prop) (m : node1*node2), transition io_aut (init io_aut) (f, g) m) as Hy.
+                (** this is given by the validInit assumption *)
+                assert (H_next_gen : next_gen (init i_aut, init o_aut) f (i0, program (i0,o_start))).
+                { 
+                    (** g and m are found using the fact that any reachable node must have a successor,
+                        so the initial output node has a successor [m] labeled by [(f,g)]
+                     *)
+                    assert (Hy : exists (g : input * state -> Prop) (m : node1*node2),
+                                transition io_aut (init io_aut) (f, g) m).
                     {
-                        assert (reachable_from o_aut (init o_aut) (init o_aut)) as H_reach by (left; reflexivity).
-                        destruct (o_aut_successors (init o_aut) H_reach) as [g [m H_trans]].
+                        assert (reachable o_aut (init o_aut)) as H_reach by (left; reflexivity).
+                        destruct (o_aut_successor (init o_aut) H_reach) as [g [m H_trans]].
                         exists g, (n1, m); easy.
                     }
-                    exact (cond_init _ _ _ _ Hy o_start_valid input_hd_is_valid).
+                    exact (cond_init _ _ _ Hy o_start_valid input_hd_is_valid).
                 }
-                destruct H_next_gen as [g [m' [H_transition_io H_g]]].
-                exists g, m'; easy.
+                destruct H_next_gen as [g [[n1' n2] [H_transition_io H_g]]].
+                exists g, n2.
+                split ; [|assumption].
+                inversion_clear H_transition_io as [_ h_transition_o].
+                exact (conj h_transition h_transition_o).
             }
-            exists (cons ((f,g), (n1,m)) nil).
+
+            exists (((f,g), (n1,m))::nil).
             split; [reflexivity|].
             split.
             +   exact (path_transition _ _ _ _ _ _ Hu). 
             +   assert (sat_product (f, g) (i0, program (i0, o_start))) as H_sat
                     by (split; [exact input_hd_is_valid | exact Hw]).
                 exact (valid_cons _ _ _ _ _ _ _ (valid_nil _ _ _) H_sat).
+
         -   subst.
-            destruct is as [ | [f_Sk n_SSk] is];
+            destruct ipath as [ | [f_Sk n_SSk] ipath];
                 [destruct input_lang as [_ Hq2]; inversion Hq2 |].
-            assert (f_Sk i_Sk) as Hp4.
+            assert (Hp4 : f_Sk i_Sk).
             {
                 destruct input_lang as [_ H_valid].
                 inversion H_valid as [ | ? ? ? ? _ H_sat]; subst.
                 exact H_sat.
             }
-            assert (language_w sat i_aut is (i_k :: inputs tr)) as input_prev_lang
+            assert (input_prev_lang : language_wit sat i_aut ipath (i_k :: inputs tr))
                 by exact (language_prefix_closed _ _ _ _ _ _ _ _ _ input_lang).
-            specialize (tr_lang o_start_valid is input_prev_lang).
+            specialize (tr_lang o_start_valid ipath input_prev_lang).
             destruct tr_lang as [p_io [H_peq [p_io_path p_io_valid]]].
             destruct p_io as [ | [[f_k g_k] [n_Sk m_Sk]] p_io]; [inversion p_io_valid|].
             assert (reachable_from io_aut (init i_aut, init o_aut) (n_Sk, m_Sk)) as Hp1.
@@ -236,7 +265,7 @@ Module Correctness (Import D : Verif_Domain).
                 }
                 assert (exists g_Sk m_SSk, transition o_aut m_Sk g_Sk m_SSk) as [g_Sk [m_SSk H_u]].
                 {
-                    apply o_aut_successors.
+                    apply o_aut_successor.
                     right.
                     exists g_k.
                     exists (List.map (fun p => (snd (fst p), snd (snd p))) p_io).
@@ -244,57 +273,41 @@ Module Correctness (Import D : Verif_Domain).
                     apply path_right_proj in p_io_path.
                     apply p_io_path.
                 }    
-                exists g_Sk, m_SSk.
-                split.
-                apply Hx.
-                apply H_u.
+                exists g_Sk, m_SSk. exact (conj Hx H_u).
             }
             
             destruct Hp2 as [g_Sk [m_SSk Hp2]].
-            assert (next_gen (n_Sk, m_Sk) f_Sk n_SSk (i_Sk, program (i_Sk, o_k))).
+            assert (next_gen (n_Sk, m_Sk) f_Sk (i_Sk, program (i_Sk, o_k))).
             {
                 apply cond_node.
                 -   apply Hp1.
-                -   exists g_Sk, (n_SSk, m_SSk).
-                    apply Hp2. (* move aux here*)
-                -   unfold prev_gen.        
-                    inversion p_io_path; subst.
-                    *   exists i_k, f_k, g_k, (init i_aut, init o_aut).
-                        split.
-                        exact H0.
-                        inversion p_io_valid; subst.
-                        apply H5.
-                    *   exists i_k, f_k, g_k, m0.
-                        split.
-                        exact H3.
-                        inversion p_io_valid; subst.
-                        apply H6.
-                -   apply Hp4.
+                -   exists g_Sk, (n_SSk, m_SSk). apply Hp2.
+                -   inversion p_io_valid as [ | ? ? ? ? Ha Hb ]; subst.
+                    inversion p_io_path as [ a  | ? ? Hc | nd ? ? ? ? ? ? Hc ]; subst.
+                    +   exists f_k, g_k, (init i_aut, init o_aut); firstorder.
+                    +   exists f_k, g_k, nd; firstorder.
+                -   exact Hp4.
             }
-            destruct H as [g_z [m_z [Hz1 Hz2]]].
+            destruct H as [g_z [[m_z1 m_z2] [Hz1 Hz2]]].
             exists (
-                cons (f_Sk, g_z, (n_SSk,m_z))
-                (cons 
-                (f_k, g_k, (n_Sk, m_Sk))
-                p_io)).
-                split.
-                *   simpl.
-                    f_equal.
-                    apply H_peq.
-                *   split.
-                    --  exact (path_transitive _ _ _ _ _ _ _ _ _ p_io_path Hz1). 
-                    --  apply valid_cons.
-                        ++  apply valid_cons.
-                            inversion p_io_valid; subst.
-                            apply H2.
-                            inversion p_io_valid; subst.
-                            apply H4.
-                        ++  split; [exact Hp4 | exact Hz2].
+                (f_Sk, g_z, (n_SSk, m_z2))::(f_k, g_k, (n_Sk, m_Sk))::p_io
+            ). 
+            simpl in *. 
+            split.
+            * f_equal. exact H_peq.
+            * split.
+                --  constructor. 
+                    + apply p_io_path.
+                    + exact (conj (proj1 Hp2) (proj2 Hz1)). 
+                --  apply valid_cons.
+                    ++  inversion p_io_valid as [ | ? ? ? ? Ha Hb]; subst.
+                            exact (valid_cons _ _ _ _ _ _ _ Ha Hb).
+                    ++  split; [exact Hp4 | exact Hz2].
     Qed.
 
     Theorem correctness : 
         forall (st : state) (tr : trace), 
-            validAutomata -> 
+            validAutomaton -> 
             D.P_init st -> run st tr -> 
             language sat i_aut (inputs tr) ->
             language sat o_aut tr.
@@ -308,12 +321,11 @@ Module Correctness (Import D : Verif_Domain).
         -   apply path_right_proj in H.
             apply H.
         -   rewrite <- temp0.
-            replace tr with (map id tr).
+            replace tr with (map id tr) by apply map_id.
             apply valid_right_proj with (sat_product := sat_product).
             intros.
             apply H1.
             apply H0.
-            apply map_id.
     Qed.
 
 End Correctness.
