coq/theories/util.v
@@ -4,3 +4,13 @@ Lemma map_id : forall (A : Type) (l : list A), map id l = l.
 Proof.
     induction l as [ | ? ? IHl]; [reflexivity| simpl; f_equal; exact IHl].
 Qed.
+
+
+
+
+Fixpoint map2 {A B C : Type} (f : A -> B -> C) (l1:list A) (l2 :list B) : list C :=
+match l1,l2 with
+    | nil,nil => nil
+    | cons a t,cons b t' => cons (f a b) (map2 f t t')
+    | _,_ => nil
+end.
